proof/refine/RISCV64/ArchInit_R.thy
@@ -1,0 +1,45 @@
+(*
+ * Copyright 2021, Data61, CSIRO (ABN 41 687 119 230)
+ *
+ * SPDX-License-Identifier: GPL-2.0-only
+ *)
+
+theory ArchInit_R
+imports
+  Init_R
+begin
+
+context Arch begin arch_global_naming
+
+named_theorems Init_R_assms
+
+definition zeroed_arch_abstract_state :: arch_state where
+  "zeroed_arch_abstract_state \<equiv> \<lparr>
+    riscv_asid_table    = Map.empty,
+    riscv_global_pts    = K {},
+    riscv_kernel_vspace = K RISCVVSpaceUserRegion\<rparr>"
+
+definition zeroed_arch_intermediate_state :: Arch.kernel_state where
+  "zeroed_arch_intermediate_state \<equiv> RISCVKernelState Map.empty (K []) (K RISCVVSpaceUserRegion)"
+
+(* the None maps are a result of unfolding zeroed_main_abstract_state *)
+lemma ghost_relation_wrapper_arch_intermediate_state[Init_R_assms]:
+  "ghost_relation_wrapper_2 (\<lambda>_. None) (\<lambda>_. None) (\<lambda>_. None) zeroed_arch_intermediate_state"
+  unfolding ghost_relation_wrapper_def ghost_relation_def zeroed_arch_intermediate_state_def
+  by simp
+
+lemma non_empty_refine_arch_state_relation[Init_R_assms]:
+  "(zeroed_arch_abstract_state, zeroed_arch_intermediate_state) \<in> arch_state_relation"
+  unfolding zeroed_arch_abstract_state_def zeroed_arch_intermediate_state_def arch_state_relation_def
+  by simp
+
+end (* Arch *)
+
+interpretation Init_R?: Init_R RISCV64.zeroed_arch_abstract_state
+                                RISCV64.zeroed_arch_intermediate_state
+proof goal_cases
+  interpret Arch  .
+  case 1 show ?case by (intro_locales; (unfold_locales; (fact Init_R_assms)?)?)
+qed
+
+end
