proof/refine/X64/ArchInit_R.thy
@@ -1,0 +1,56 @@
+(*
+ * Copyright 2021, Data61, CSIRO (ABN 41 687 119 230)
+ *
+ * SPDX-License-Identifier: GPL-2.0-only
+ *)
+
+theory ArchInit_R
+imports
+  Init_R
+begin
+
+context Arch begin arch_global_naming
+
+named_theorems Init_R_assms
+
+definition zeroed_arch_abstract_state :: arch_state where
+  "zeroed_arch_abstract_state \<equiv> \<lparr>
+    x64_asid_table         = Map.empty,
+    x64_global_pml4        = 0,
+    x64_kernel_vspace      = K X64VSpaceUserRegion,
+    x64_global_pts         = [],
+    x64_global_pdpts       = [],
+    x64_global_pds         = [],
+    x64_current_cr3        = cr3 0 0 ,
+    x64_allocated_io_ports = \<bottom>,
+    x64_num_ioapics        = 0,
+    x64_ioapic_nirqs       = K 0,
+    x64_irq_state          = K IRQFree,
+    x64_current_fpu_owner = None\<rparr>"
+
+definition zeroed_arch_intermediate_state :: Arch.kernel_state where
+  "zeroed_arch_intermediate_state \<equiv>
+     X64KernelState Map.empty 0 [] [] [] (CR3 0 0)
+                    (K X64VSpaceUserRegion) \<bottom> 0 (K 0) (K X64IRQFree) None"
+
+(* the None maps are a result of unfolding zeroed_main_abstract_state *)
+lemma ghost_relation_wrapper_arch_intermediate_state[Init_R_assms]:
+  "ghost_relation_wrapper_2 (\<lambda>_. None) (\<lambda>_. None) (\<lambda>_. None) zeroed_arch_intermediate_state"
+  unfolding ghost_relation_wrapper_def ghost_relation_def zeroed_arch_intermediate_state_def
+  by simp
+
+lemma non_empty_refine_arch_state_relation[Init_R_assms]:
+  "(zeroed_arch_abstract_state, zeroed_arch_intermediate_state) \<in> arch_state_relation"
+  unfolding zeroed_arch_abstract_state_def zeroed_arch_intermediate_state_def arch_state_relation_def
+  by (simp add: cr3_relation_def x64_irq_relation_def comp_def)
+
+end (* Arch *)
+
+interpretation Init_R?: Init_R X64.zeroed_arch_abstract_state
+                                X64.zeroed_arch_intermediate_state
+proof goal_cases
+  interpret Arch  .
+  case 1 show ?case by (intro_locales; (unfold_locales; (fact Init_R_assms)?)?)
+qed
+
+end
